proof/invariant-abstract/SchedContextInv_AI.thy
@@ -1532,7 +1532,11 @@ lemma charge_budget_invs[wp]:
       apply (wpsimp wp: end_timeslice_invs assert_inv hoare_vcg_if_lift2 gts_wp
                         hoare_vcg_all_lift  sc_consumed_add_invs refill_budget_check_invs
                   simp: Let_def)+
-  done
+apply (frule invs_cur)
+apply (auto split: if_splits kernel_object.splits thread_state.splits simp: schedulable_def get_tcb_def opt_map_def obj_at_def ct_in_state_def pred_tcb_at_def
+cur_tcb_def is_tcb_def)
+  apply (meson kernel_object.exhaust)
+  by (metis (no_types, lifting) option.case_eq_if runnable_eq)
 
 lemma check_budget_invs[wp]:
   "\<lbrace>\<lambda>s. invs s\<rbrace> check_budget \<lbrace>\<lambda>rv. invs \<rbrace>"
